CoqCode/Soundness.v
@@ -1,75 +1,138 @@
 Require Import Metalib.Metatheory.
 Require Import Coq.Program.Equality.
-Require Import Language Subtyping Notations.
+Require Import Language Subtyping Auxiliaries Notations Deterministic.
 
-Inductive runsub : typ -> typ -> Prop :=
-| rsub_refl : forall (A : typ),
-    runsub A A
-| rsub_arrow : forall (A1 A2 B1 B2 : typ),
-    sub B1 A1 -> runsub A2 B2 ->
-    runsub (typ_arrow A1 A2) (typ_arrow B1 B2)
-| rsub_and : forall (A1 A2 B1 B2 : typ),
-    runsub A1 B1 -> runsub A2 B2 ->
-    runsub (typ_and A1 A2) (typ_and B1 B2)
-| rsub_top : forall (A : typ),
-    toplike A -> runsub typ_top A.
+Lemma sub_ord_disjoint :
+  forall (A B C : typ),
+    ordinary C -> disjoint_spec A B -> sub (typ_and A B) C ->
+    sub A C /\ sub B C.
+Proof.
+  intros A B C Hord Hdisj Hsub.
+  dependent destruction Hsub; try solve [inversion Hord].
+  - split; eauto.
+  - assert (Htl: toplike (typ_arrow B1 B2)).
+    constructor. eapply toplike_sub_top; eauto.
+    split; eauto.
+Admitted.
 
 Theorem tred_preservation :
   forall (v v' : trm) (A: typ),
-    value v -> typing nil nil check_mode v A ->
+    value v ->
+    typing nil nil check_mode v A ->
     typedred v A v' ->
-    exists (B : typ), typing nil nil infer_mode v' B /\ runsub B A.
+    typing nil nil infer_mode v' A.
 Proof.
-  intros v v' A B.
-  intros Htyp Hred.
+  intros v v' A Hv Htyp Hred.
   dependent induction Hred.
-  - exists typ_int. split.
-    + apply typing_anno.
-      apply as_refl.
-      apply typing_sub with (B:=typ_int).
-      apply typing_int. constructor. apply sub_reflexivity.
-    + apply rsub_refl.
-  - exists typ_top. split.
-    + apply typing_anno.
-      apply as_refl.
-      apply typing_sub with (B:=typ_top).
-      apply typing_top. apply sub_reflexivity.
-    + apply rsub_top. assumption.
-  - exists (typ_arrow A D). split.
-    Focus 2.
-    + apply rsub_arrow. assumption. apply rsub_refl.
-    + apply typing_anno.
-      apply as_refl.
-      inversion Htyp; subst; clear Htyp.
-      inversion H2; subst; clear H2.
-      inversion H8; subst; clear H8.
-      inversion H3; subst.
-      Focus 2.
-      eapply typing_abs1.
-      intros.
-      (* inversion Htyp; subst. inversion H3; subst. *)
-      (* inversion H10; subst. *)
-      (* specialize (H11 x). *)
+  - eapply typing_anno; eauto.
+  - eapply typing_anno; eauto.
+    admit. (* appsub and toplike *)
+  - apply typing_anno; eauto.
+    dependent destruction Htyp.
+    dependent destruction Htyp.
+    eapply typing_sub_check; eauto.
+  - dependent destruction Hv.
+    dependent destruction Htyp.
+    dependent destruction Htyp.
+    + apply IHHred; eauto.
+      eapply typing_sub.
+      apply Htyp1. (* Tred-Merge-L *)
+      admit.
+    + apply IHHred; eauto.
+      eapply typing_sub.
+      eapply Htyp1.
+      admit.
+  - dependent destruction Hv.
+    dependent destruction Htyp.
+    dependent destruction Htyp.
+    + apply IHHred; eauto.
+      eapply typing_sub.
+      apply Htyp2.
+      admit.
+    + apply IHHred; eauto.
+      eapply typing_sub.
+      apply Htyp2.
+      admit.
+  - eapply typing_merge_value.
+    + eapply tred_value; eauto.
+    + eapply tred_value; eauto.
+    + eapply IHHred1. assumption.
+      admit.
+    + eapply IHHred2. assumption.
+      admit.
+    + eapply tred_consistency; eauto.
+Admitted.
+
+Lemma papp_preservation :
+  forall (r v e : trm) (A B : typ) (S : arg),
+    rvalue r -> value v ->
+    papp r v e ->
+    typing nil nil infer_mode v A ->
+    typing nil (cons A S) infer_mode r (typ_arrow A B) ->
+    typing nil S infer_mode e B.
+Proof.
+  intros r v e A B Hr Hv Hp Htyp1 Htyp2.
+  generalize dependent A.
+  generalize dependent B.
+  dependent induction Hp; intros.
+Admitted.
+
+Lemma papp_preservation_check :
+  forall (r v e : trm) (A B : typ),
+    rvalue r -> value v ->
+    papp r v e ->
+    typing nil nil infer_mode v A ->
+    typing nil nil check_mode r (typ_arrow A B) ->
+    typing nil nil check_mode e B.
+Proof.
 Admitted.
 
 Theorem preservation :
-  forall (e e' : trm) (A : typ),
-    typing nil nil infer_mode e A ->
+  forall (e e' : trm) (A : typ) (dir : mode) (S : arg),
+    typing nil S dir e A ->
     step e e' ->
-    typing nil nil check_mode e' A.
+    typing nil S dir e' A.
 Proof.
-  intros e e' A Htyp Hred.
-  induction Htyp.
-  - inversion Hred; subst.
-    apply typing_sub with (B:=typ_int).
-    apply typing_anno. constructor.
-    apply typing_sub with (B:=typ_int).
-    apply typing_int. assumption. apply sub_reflexivity. apply sub_reflexivity.
-  - inversion Hred.
-  - inversion Hred.
-  - inversion Hred.
-  - inversion Hred.
-  - inversion Hred; subst.
-    + induction A; eauto.
-      * inversion H; subst; clear H.
+  intros e e' A dir S Htyp Hred.
+  generalize dependent e'.
+  dependent induction Htyp; intros.
+  - dependent destruction Hred.
+    eapply typing_anno; eauto.
+  - dependent destruction Hred.
+  - dependent destruction Hred.
+  - dependent destruction Hred.
+  - dependent destruction Hred.
+  - dependent destruction Hred.
+  - dependent destruction Hred.
+    + assert (Htyp2: typing nil nil infer_mode v' A).
+      eapply tred_preservation; eauto.
+      admit.
+    + eapply typing_anno. assumption.
+      eapply IHHtyp; eauto.
+  - dependent destruction Hred.
+    + eapply papp_preservation; eauto.
+    + eapply typing_app1; eauto.
+    + eapply typing_app1; eauto.
+  - dependent destruction Hred.
+    + eapply papp_preservation_check; eauto.
+    + eapply typing_app2; eauto.
+    + eapply typing_app2; eauto.
+  - assert (Htyp2: typing nil nil infer_mode e' B).
+    eapply IHHtyp; eauto.
+    eapply typing_sub; eauto.
+  - dependent destruction Hred.
+    + eapply typing_merge; eauto.
+    + eapply typing_merge; eauto.
+  - assert (Hval: value (trm_merge v1 v2)).
+    constructor; eauto.
+    apply value_cannot_step_further with (e:=e') in Hval.
+    destruct Hval. assumption.
+  - assert (Htyp2: typing nil S infer_mode e' B).
+    eapply IHHtyp; eauto.
+    dependent destruction Hred.
+    (*
+      The problem is
+      reduction of merge picking appears at papp
+      typing of merge picking appears at merge
+     *)
 Admitted.
